update definition: <OP x v | \phi >

formalization/Equation.v
@@ -10,28 +10,30 @@ Import NamelessTactics.
 Inductive trace : Type :=
 | ϵ
 | trretv (v: value)
-| trevent (op: effop) (v: value)
-| trseq (op: effop) (v: value) (tr: trace).
+| trseq (op: effop) (argv: constant) (retv: constant) (tr: trace).
 
 Coercion trretv : value >-> trace.
 
-Notation " op ':{' v  '}' " := (trevent op v) (at level 20, op constr, v constr, right associativity).
+Notation " 'tr{' op ',' v1 ',' v2 '}' " := (trseq op v1 v2 ϵ)
+                                        (at level 20, format "tr{ op , v1 , v2 }",
+                                          op constr, v1 constr, v2 constr, right associativity).
 
-Notation " op ':{' v  '};' e" := (trseq op v e) (at level 20, op constr, v constr, e constr, right associativity).
+Notation " 'tr{' op ',' v1 ',' v2 '}::' α " := (trseq op v1 v2 α)
+                                        (at level 20, format "tr{ op , v1 , v2 }:: α",
+                                          op constr, v1 constr, v2 constr, right associativity).
 
 Fixpoint trace_app (tr1 tr2: trace): trace :=
   match tr1 with
   | ϵ => tr2
   | trretv _ => tr2
-  | trevent op v => op :{ v }; tr2
-  | (trseq op v tr1) => op :{ v }; (trace_app tr1 tr2)
+  | tr{ op, v1, v2 }:: α => tr{ op , v1, v2 }:: (trace_app α tr2)
   end.
 
 Notation " a '+;+' b" := (trace_app a b) (at level 20, a constr, b constr, right associativity).
 
 Inductive with_retv: trace -> Prop :=
 | with_retv_retv: forall v, with_retv (trretv v)
-| with_retv_seq: forall op v e, with_retv e -> with_retv (op :{ v }; e).
+| with_retv_seq: forall op v1 v2 e, with_retv e -> with_retv (tr{ op,  v1, v2 }:: e).
 
 Theorem tr_app_ϵ_end : forall tr, tr = tr +;+ ϵ.
 Admitted.
@@ -47,27 +49,31 @@ Proof.
     auto using tr_app_ass.
 Qed.
 
-Theorem tr_app_comm_cons : forall x y op v, op :{ v }; (x +;+ y) = (op :{ v }; x) +;+ y.
+Theorem tr_app_comm_cons : forall x y op v1 v2, tr{ op, v1 , v2 }:: (x +;+ y) = (tr{ op, v1, v2 }:: x) +;+ y.
 Proof.
   auto.
 Qed.
 
-Theorem tr_app_cons_not_ϵ : forall x y op v, ϵ <> x +;+ op :{v}; y.
+Theorem tr_app_cons_not_ϵ : forall x y op v1 v2, ϵ <> x +;+ tr{op, v1, v2}:: y.
 Admitted.
 
 Theorem tr_app_eq_ϵ : forall l l', l +;+ l' = ϵ -> l = ϵ  /\ l' = ϵ .
 Admitted.
 
 Theorem app_eq_unit :
-    forall x y op a,
-      x +;+ y = op :{a}; ϵ -> x = ϵ /\ y = op :{a}; ϵ \/ x = op :{a}; ϵ /\ y = ϵ.
+    forall x y op v1 v2,
+      x +;+ y = tr{op, v1, v2} -> x = ϵ /\ y = tr{ op, v1, v2} \/ x = tr{ op, v1, v2} /\ y = ϵ.
 Admitted.
 
 Lemma app_inj_tail :
-    forall (x y:trace) op_a op_b (a b: value), x +;+ op_a :{a}; ϵ = y +;+ op_b :{b}; ϵ -> x = y /\ a = b.
+    forall (x y:trace) op_a op_b (a1 a2 b1 b2: constant),
+      x +;+ tr{op_a, a1, a2} = y +;+ tr{op_b, b1, b2} -> x = y /\ a1 = b1 /\ a2 = b2.
 Admitted.
 
-Definition tr_reduction: trace -> trace -> Prop.
+Definition tr_reduction: trace -> effop -> constant -> constant -> Prop.
 Admitted.
 
-Notation " a '⇓' b" := (tr_reduction a b) (at level 30, a constr, b constr).
+Notation " 'app{' op ',' c1 '}⇓{' α '}' c" := (tr_reduction α op c1 c)
+                                          (at level 30, format "app{ op , c1 }⇓{ α } c", c1 constr, α constr).
+
+
